Bound adversary success with stat distance

stat-dist.ec
@@ -273,6 +273,22 @@ op adv_distr : bits -> bool distr.
 
 axiom is_adv_distr &m (x : bits) (b : bool): (Pr[Adv.guess(x) @ &m : res = b]) = mu1 (adv_distr x) b.
 
+lemma adv_distr_ll &m (x : bits) : is_lossless (adv_distr x).
+proof.
+rewrite /is_lossless.
+(*have -> : weight (adv_distr x) = mu (adv_distr x) predT.*)
+have -> : predT = predU (pred1 true) (pred1 false).
+rewrite /predT /predU /pred1 fun_ext /(==) => b0; case b0; progress.
+rewrite mu_disjoint.
+rewrite /predI /pred1 /pred0 /(<=) => a; case a; progress.
+rewrite -(is_adv_distr &m) -(is_adv_distr &m).
+have -> : (Pr[Adv.guess(x) @ &m : res = true] + Pr[Adv.guess(x) @ &m : res = false]) = Pr[Adv.guess(x) @ &m : res = true \/ res = false].
+rewrite Pr[mu_disjoint]; progress; case (res{hr}); progress.
+have -> : Pr[Adv.guess(x) @ &m : res = true \/ res = false] = Pr[Adv.guess(x) @ &m : true].
+rewrite Pr[mu_eq]; progress; case (res{hr}); progress.
+byphoare; trivial. by exact Adv_ll.
+qed.
+
 op da : bits distr.
 
 axiom da_ll : is_lossless da.
@@ -282,6 +298,9 @@ op db : bits distr.
 axiom db_ll : is_lossless db.
 
 
+op select_d : bool -> bits distr = (fun (b : bool) => if !b then da else db).
+
+
 local module Exp = {
 
   proc main() : bool = {
@@ -289,7 +308,7 @@ local module Exp = {
     var d : bits distr;
     var x : bits;
     b <$ {0,1};
-    d <- if !b then da else db;
+    d <- select_d(b);
     x <$ d;
     ba <- Adv.guess(x);
     return ba = b;
@@ -298,6 +317,8 @@ local module Exp = {
 
 
 module Sampling = {
+ 
+  var x : bits
 
   proc sample(x : bits) : bool = {
     var b_ : bool;
@@ -305,15 +326,20 @@ module Sampling = {
     return b_;
   }
 
-  proc main() : bool = {
-    var b, ba : bool;
+  proc select(b : bool) : bool = {
+    var ba : bool;
     var d : bits distr;
-    var x : bits;
-    b <$ {0,1};
-    d <- if !b then da else db;
+    d <- select_d(b);
     x <$ d;
     ba <@ sample(x);
     return ba = b;
+  }
+
+  proc main() : bool = {
+    var b, r : bool;
+    b <$ {0,1};
+    r <@ select(b);
+    return r;
   }
 }.
 
@@ -321,8 +347,10 @@ module Sampling = {
 local lemma adv_distr_eq : equiv[Exp.main ~ Sampling.main : true ==> ={res}].
 proof.
 proc.
-seq 3 3 : (={b, d, x}).
+inline Sampling.select.
+seq 3 4 : (={b, d} /\ x{1} = Sampling.x{2} /\ b0{2} = b{2}).
 rnd; wp; rnd; skip; progress.
+wp.
 call (: ={x} ==> ={res}).
 bypr (res){1} (res){2} => //=.
 progress.
@@ -336,63 +364,138 @@ trivial.
 skip. progress.
 qed.
 
-op support_fst : bits = head witness Support.enum.
+(*op support_fst : bits = head witness Support.enum.*)
 
 
-lemma disting_false: (forall (x : bits ), x \in Support.enum) => (phoare [Sampling.main : true ==> res] = ((inv 2%r * big predT (fun x => mu1 (adv_distr x) false * mu1 da x) Support.enum) + (inv 2%r * big predT (fun x => mu1 (adv_distr x) true * mu1 db x) Support.enum))).
+lemma dist_select (b_quant : bool): uniq Support.enum => phoare [Sampling.select : b = b_quant ==> res /\ Sampling.x \in Support.enum] = (big predT (fun x_ => mu1 (adv_distr x_) b_quant * mu1 (select_d b_quant) x_) Support.enum).
 proof.
-
-lemma disting0: (forall (x : bits ), x \in Support.enum) => (phoare [Sampling.main : true ==> res] = ((inv 2%r * big predT (fun x => mu1 (adv_distr x) false * mu1 da x) Support.enum) + (inv 2%r * big predT (fun x => mu1 (adv_distr x) true * mu1 db x) Support.enum))).
-proof.
-move => ?.
-
-proc.
-seq 1 : (b = false) (inv 2%r) ( big predT (fun x => mu1 (adv_distr x) false * mu1 da x) Support.enum) (inv 2%r) (big predT (fun x => mu1 (adv_distr x) true * mu1 db x) Support.enum) true.
-rnd; skip; progress.
-rnd; skip; progress; rewrite dboolE_count => //=; rewrite /b2i => //=.
-
-elim Support.enum. auto.
+elim: Support.enum => [ //= |x_bits lst ih]. rewrite big_nil; auto.
+move => is_uniq.
+simplify.
+phoare split (mu1 (adv_distr x_bits) b * mu1 (select_d b) x_bits) (big predT (fun (x_ : bits) => mu1 (adv_distr x_) b_quant * mu1 (select_d b_quant) x_) lst) : (Sampling.x = x_bits).
 progress.
 proc.
+sp; inline Sampling.sample; wp.
+seq 1 : (Sampling.x = x_bits) (mu1 (select_d b) x_bits) (mu1 (adv_distr x_bits) b) (1%r - mu1 (select_d b) x_bits) 0%r => //=.
+rnd; skip; progress.
+sp; rnd; skip; progress.
+sp; rnd; skip; progress.
+rewrite mu0_false; progress; rewrite negb_and; left; assumption.
+progress; algebra.
+conseq (: b = b_quant ==> res /\ Sampling.x \in lst).
+progress.
+elim H1. progress. apply implyFb; apply H.
+trivial.
+elim is_uniq => x_not_in uniq_list {uniq_list}.
+apply (contraNneq (x_bits \in lst)). move => x_x_bit_eq.
+rewrite -x_x_bit_eq; assumption. assumption.
+right; assumption.
+apply ih.
+elim is_uniq. trivial.
+qed.
+
+(*lemma dist_select &m (b_par : bool): uniq Support.enum => Pr [Sampling.select(b_par) @ &m: res /\ Sampling.x \in Support.enum] = (big predT (fun x_ => mu1 (adv_distr x_) b_par * mu1 (select_d b_par) x_) Support.enum).
+proof.
+elim: Support.enum => [ //= |x_bits lst ih]. rewrite big_nil.
+byphoare; auto.
+move => is_uniq.
+simplify.
+rewrite andb_orr.
+rewrite Pr [mu_disjoint].
+smt.
+rewrite ih. elim is_uniq; trivial.
+have -> : Pr[Sampling.select(b_par) @ &m : res /\ Sampling.x = x_bits] = (mu1 (adv_distr x_bits) b_par) * mu1 (select_d b_par) x_bits.
+byphoare (: b{hr} = b_par ==>  res /\ Sampling.x = x_bits).
+proc.
+sp.
+inline Sampling.sample.
+wp.
+seq 1 : (Sampling.x = x_bits) (mu1 (select_d b) x_bits) (mu1 (adv_distr x_bits) b) (1%r - mu1 (select_d b) x_bits) 0%r => //=.
+rnd; skip; progress. 
+sp.
+rnd; skip; progress.
+sp; rnd; skip; progress.
+have isF : ((fun (x : bool) => x = b{hr} /\ Sampling.x{hr} = x_bits)) = fun (x : bool) => false.
+rewrite fun_ext /(==); move => bb.
+rewrite neqF negb_and. right; assumption.
+rewrite isF. apply mu0_false; simplify; auto.
+progress.
+smt. trivial. trivial.
+auto.
+qed.*)
+
+lemma disting_exact: phoare [Sampling.main : true ==> res] = ((inv 2%r * big predT (fun x => mu1 (adv_distr x) false * mu1 da x) Support.enum) + (inv 2%r * big predT (fun x => mu1 (adv_distr x) true * mu1 db x) Support.enum)).
+proof.
+proc.
 seq 1 : (b = false) (inv 2%r) ( big predT (fun x => mu1 (adv_distr x) false * mu1 da x) Support.enum) (inv 2%r) (big predT (fun x => mu1 (adv_distr x) true * mu1 db x) Support.enum) true.
 rnd; skip; progress.
 rnd; skip; progress; rewrite dboolE_count => //=; rewrite /b2i => //=.
-sp.
-
-
-
-rnd (x = support_fst) (mu1 da x) (mu1 (adv_distr x) false) (inv 2%r) 1%r => //=. 
-call (: true ==> true) (inv 2%r).
-proc.
-rnd; skip => //=.
-
-phoare split (
-  inv 2%r * big predT (fun (x0 : bits) => Pr[Adv.guess(x0) @ &m : false] * mu1 da x0) Support.enum
-) (
-  inv 2%r * big predT (fun (x0 : bits) => Pr[Adv.guess(x0) @ &m : true] * mu1 db x0) Support.enum
-) : (!Exp.b) => //.
-(*seq 2 : (!Exp.b /\ d = da) (inv 2%r) (big predT (fun (x0 : bits) => Pr[Adv.guess(x0) @ &m : false] * mu1 da x0) Support.enum) (inv 2%r) 0%r.*)
-admit. admit.
+call (dist_select false). by exact/Support.enum_uniq.
+skip; progress. by exact Support.enumP.
+rnd; skip; progress.
+rewrite dboolE_count => //=; rewrite /b2i => //=.
+conseq (: b = true ==> r); progress. rewrite neqF in H. rewrite eqT negbNE; assumption.
+call (dist_select true). by exact/Support.enum_uniq.
+skip; progress. by exact Support.enumP.
+trivial.
 qed.
 
 
-
-lemma disting &m : Pr[Exp(Adv).main() @ &m : res] <= inv 2%r * (1%r + delta_d da db).
-proof.
-byphoare.
-proc.
-(*call (_ : b = b ==> b = b').
-seq 1 : ((b \in {0,1}) /\ mu1 dbool b = inv 2%r).
-rnd. skip. auto.
-rnd. skip.
-call (_ : true ==> true).
-seq 3 : true.
-call (_ : true ==> true).
-apply Adv_ll.
-seq 1 : true.
-rnd.
-skip. auto.*)
-admit. admit. admit.
+lemma disting_delta_bound : phoare [Sampling.main : true ==> res] <= ((inv 2%r) * (1%r + delta_d da db)).
+bypr.
+move => &m true_ {true_}.
+have -> : Pr[Sampling.main() @ &m : res] = ((inv 2%r * big predT (fun x => mu1 (adv_distr x) false * mu1 da x) Support.enum) + (inv 2%r * big predT (fun x => mu1 (adv_distr x) true * mu1 db x) Support.enum)).
+byphoare disting_exact; trivial.
+pose x_false_s := big predT (fun (x : bits) => mu1 (adv_distr x) false * mu1 da x) Support.enum.
+pose x_true_s := big predT (fun (x : bits) => mu1 (adv_distr x) true * mu1 db x) Support.enum.
+have -> : (inv 2%r * x_false_s + inv 2%r * x_true_s <= inv 2%r * (1%r + delta_d da db)) <=> (x_false_s + x_true_s <= (1%r + delta_d da db)).
+smt.
+rewrite /x_false_s /x_true_s.
+rewrite delta_d_alt. exact da_ll. by exact db_ll.
+have adv_ft : forall (x : bits), mu1 (adv_distr x) true = 1%r - mu1 (adv_distr x) false.
+move => x.
+rewrite -subr_eq opprK.
+rewrite -mu_disjoint /pred0 /predI /pred1 /(<=) => //=.
+move => a. rewrite negb_and; case a; progress.
+rewrite /predU.
+have -> : (fun (x0 : bool) => x0 = true \/ x0 = false) = predT.
+rewrite fun_ext /(==) => x0; rewrite /predT; case x0; progress.
+exact (adv_distr_ll &m).
+have -> : (fun (x : bits) => mu1 (adv_distr x) true * mu1 db x) = fun (x : bits) => mu1 db x - mu1 (adv_distr x) false * mu1 db x.
+rewrite fun_ext /(==) => x.
+rewrite adv_ft. smt.
+rewrite big_split.
+have -> : big predT (fun (i : bits) => mu1 db i) Support.enum = 1%r.
+have -> : big predT (fun (i : bits) => mu1 db i) Support.enum = weight db.
+rewrite muE. rewrite (sumE_fin<:bits> (fun (x : bits) => if predT x then mass db x else 0%r) (Support.enum)). exact Support.enum_uniq. progress. exact Support.enumP.
+have -> : (fun (x : bits) => mass db x) = fun (i : bits) => mu1 db i.
+rewrite /predT fun_ext /(==) => x; simplify. rewrite massE. trivial. trivial.
+exact db_ll.
+rewrite -/x_false_s.
+have -> : (x_false_s + (1%r + big predT (fun (i : bits) => - mu1 (adv_distr i) false * mu1 db i) Support.enum) <= 1%r + big (fun (x : bits) => mu1 db x < mu1 da x) (fun (x : bits) => mu1 da x - mu1 db x) Support.enum) <=> (x_false_s + big predT (fun (i : bits) => - mu1 (adv_distr i) false * mu1 db i) Support.enum <=
+big (fun (x : bits) => mu1 db x < mu1 da x)
+  (fun (x : bits) => mu1 da x - mu1 db x) Support.enum).
+smt.
+rewrite /x_false_s.
+rewrite -big_split => //=.
+have -> : (fun (i : bits) => mu1 (adv_distr i) false * mu1 da i - mu1 (adv_distr i) false * mu1 db i) = fun (x : bits) => mu1 (adv_distr x) false * (mu1 da x - mu1 db x).
+rewrite fun_ext /(==) => x. rewrite mulrDr mulrN; trivial.
+apply (ler_trans (big predT (fun (x : bits) => if mu1 db x < mu1 da x then mu1 (adv_distr x) false * (mu1 da x - mu1 db x) else 0%r) Support.enum)).
+apply ler_sum. rewrite /predT => //=. move => a.
+case (mu1 db a < mu1 da a); trivial.
+move => db_db_nl.
+smt (ge0_mu).
+rewrite -big_mkcond.
+apply ler_sum => //= => x mu1_db_lt_da.
+smt (ge0_mu).
 qed.
+
+
+local lemma adv_success_bound &m : Pr[Exp.main() @ &m : res] <= ((inv 2%r) * (1%r + delta_d da db)).
+have -> : Pr[Exp.main() @ &m : res] = Pr[Sampling.main() @ &m : res].
+byequiv; auto. conseq (: true ==> ={res}); auto. exact adv_distr_eq.
+byphoare; trivial; exact disting_delta_bound.
+qed.
+
 end section.
 
